\documentclass[\string~/GitHub/sthlmNordBeamerTheme/sthlmNordLightDemo.tex]{subfiles}

\begin{document}
    
    %   FRAME START   --==-=-=-=-=-=-=-=-=-=-=-=-=-=-=-=-=-=-=-=-=-=-=-=-=-=-=-=-=-=-=
    \begin{frame}[allowframebreaks, allowdisplaybreaks, t, fragile]{Implementation}{Mathematical Expression}
        \remarks Since $u$ and $v$ have the same mathematical expression, and are only different in notation. Let us use $u$ for now.
        
        Consider the general procedure for x-component velocity $u$ such that: \begin{equation}
            \begin{split}
                \frac{\Hat{u}^k - \Hat{u}^{k-1}}{\Delta t} = (\alpha_k + \beta_k) L \left( \Hat{u}^{k-1} \right) &- \frac{\alpha_k}{\mathcal{Re}} \frac{\delta}{\delta x} \left( \frac{\delta \Hat{u}^{k-1}}{\delta x} + \frac{\delta \Hat{v}^{k-1}}{\delta y}  \right) \\
                &+ \beta_k L \left( \Hat{u}^k - \Hat{u}^{k-1} \right) - \gamma_k N \left( u^{* k-1} \right) - \zeta_k N \left( u^{* k-2} \right)
            \end{split}
            \label{eq:LeMoin-1}
        \end{equation}

        \begin{equation}
            \frac{u^{*k} - \Hat{u}^k}{\Delta t} = - \frac{\delta \Phi^{*k}_x}{\delta x}
            \label{eq:LeMoin-2}
        \end{equation}

        \framebreak

        Substituting the expression for the viscous terms $L(u)$ and convective term $N(u)$ into eq. (\ref{eq:LeMoin-1}), one can achieve the following:
        \begin{equation}
            \begin{split}
                \Hat{u}^k = \Hat{u}^{k-1} &+ \frac{\Delta t}{\mathcal{Re}} (\alpha_k + \beta_k) \left( \frac{\delta^2 \Hat{u}^{k-1}}{\delta x^2} + \frac{\delta^2 \Hat{u}^{k-1}}{\delta y^2} \right) \\
                    &- \frac{\alpha_k \Delta t }{\mathcal{Re}} \frac{\delta}{\delta x} \left( \frac{\delta \Hat{u}^{k-1}}{\delta x} + \frac{\delta \Hat{v}^{k-1}}{\delta y}  \right) \\
                    &+ \frac{\beta_k \Delta t }{\mathcal{Re}} \left[ \frac{\delta^2 \left( \Hat{u}^k - \Hat{u}^{k-1} \right)}{\delta x^2} + \frac{\delta^2 \left( \Hat{u}^k - \Hat{u}^{k-1} \right)}{\delta y^2} \right] \\
                    &- \gamma_k \Delta t  \left( \frac{\delta }{\delta x} u^{* k-1} u^{* k-1} + \frac{\delta }{\delta y} u^{* k-1} v^{* k-1} \right) \\
                    &- \zeta_k \Delta t  \left( \frac{\delta }{\delta x} u^{* k-2} u^{* k-2} + \frac{\delta }{\delta y} u^{* k-2} v^{* k-2} \right) 
            \end{split}
        \end{equation}
        
    \end{frame}
    %   FRAME END   --==-=-=-=-=-=-=-=-=-=-=-=-=-=-=-=-=-=-=-=-=-=-=-=-=-=-=-=-=-=-=
    
\end{document}